language_formalisation/operational_semantics/operational_semantics.v
@@ -1,33 +1,33 @@
-Add LoadPath "C:\Users\Ziga\Documents\Ziga_podatki\PHD\language_formalisation\syntax".
-Add LoadPath "C:\Users\Ziga\Documents\Ziga_podatki\PHD\language_formalisation\substitution".
-(* Add Rec LoadPath "E:\Ziga_Podatki\faks\PHD\language_formalisation\syntax". *)
-(* Add Rec LoadPath "E:\Ziga_Podatki\faks\PHD\language_formalisation\substitution". *)
+(* Add LoadPath "C:\Users\Ziga\Documents\Ziga_podatki\PHD\language_formalisation\syntax". *)
+(* Add LoadPath "C:\Users\Ziga\Documents\Ziga_podatki\PHD\language_formalisation\substitution". *)
+Add Rec LoadPath "E:\Ziga_Podatki\faks\PHD\language_formalisation\syntax".
+Add Rec LoadPath "E:\Ziga_Podatki\faks\PHD\language_formalisation\substitution".
 Require Export syntax substitution.
 
 Inductive step : comp -> comp -> Prop :=
 | Step_ΠMatch v1 v2 x y c: 
     step 
       (ΠMatch (Pair v1 v2) x y c)
-      (c_sub2_out c v1 v2)
+      (c_subs2_out c v1 v2)
 | Step_ΣMatch_Inl v xl cl xr cr:
     step 
       (ΣMatch (Inl v) xl cl xr cr)
-      (c_sub_out cl v)
+      (c_subs_out cl v)
 | Step_ΣMatch_Inr v xl cl xr cr:
     step 
       (ΣMatch (Inr v) xl cl xr cr)
-      (c_sub_out cr v)
+      (c_subs_out cr v)
 | Step_App x c v:
-    step (App (Fun x c) v) (c_sub_out c v)
+    step (App (Fun x c) v) (c_subs_out c v)
 | Step_LetRec f x c1 c2:
     step
       (LetRec f x c1 c2)
-      (c_sub_out c2 (Fun x (LetRec f x (Sub.c_shift c1 1 2) c1)))
+      (c_subs_out c2 (Fun x (LetRec f x (Sub.c_shift c1 1 2) c1)))
 | Step_DoBind_step x c1 c1' c2:
     step c1 c1' ->
     step (DoBind x c1 c2) (DoBind x c1' c2)
 | Step_DoBind_Ret x v c:
-    step (DoBind x (Ret v) c) (c_sub_out c v)
+    step (DoBind x (Ret v) c) (c_subs_out c v)
 | Step_DoBind_Op x op_id v_arg y c1 c2:
     step
       (DoBind x (Op op_id v_arg y c1) c2)
@@ -38,12 +38,12 @@ Inductive step : comp -> comp -> Prop :=
 | Step_Handle_Ret x c_r h v :
     step
       (Handle (Handler x c_r h) (Ret v))
-      (c_sub_out c_r v)
+      (c_subs_out c_r v)
 | Step_Handle_Op x c_r h op_id v_arg y c_k x_op k_op c_op :
     find_op_case h op_id = Some (x_op, k_op, c_op) ->
     step
       (Handle (Handler x c_r h) (Op op_id v_arg y c_k))
-      (c_sub2_out c_op
+      (c_subs2_out c_op
         (Fun y (Handle (Sub.v_shift (Handler x c_r h) 1 0) c_k))
         v_arg )
 .
